Updated background theory and BoogiePL generation for new Boogie syntax. Added Routine functions to background theory. Added generation for Agent creation. Added mapping for type BOOLEAN. Added simple frame condition to all functions for agent preservation. Parsing of Boogie output made more robust. When verifying a class, project will automatically be compiled first. Ported generation of frame condition byte nodes from Ballet 5.7.

ballet/63/Src/ballet/background_theory.bpl
@@ -7,40 +7,67 @@
 // STATE
 
 // Some things are heaps
-function IsHeap(h:[ref,name]any) returns (bool);
+function IsHeap(heap:[ref,<x>name]x) returns (bool);
 
-// Given an heap, some things are allocated
-const unique $allocated:name;
-function IsAllocated(h: [ref,name]any, o: any) returns (bool);
-axiom (forall h: [ref,name]any, o: ref ::
-        IsAllocated(h,o) <==> cast(h[o,$allocated],bool));
+// Given a heap, some things are allocated
+const unique $allocated: <bool>name;
+function IsAllocated(heap: [ref,<x>name]x, o: any) returns (bool);
+//axiom (forall heap: [ref,<x>name]x, o: ref ::
+//            { IsAllocated(heap, o) } // Trigger
+//        IsAllocated(heap,o) <==> cast(heap[o,$allocated],bool));
 
 // Every reference stored in the heap is allocated
-axiom (forall h:[ref,name]any, o: ref, f: name :: 
-	{ IsAllocated(h,h[o,f]) }
-	IsHeap(h) ==> IsAllocated(h,h[o,f]));
+axiom (forall heap: [ref,<x>name]x, o: ref, f: name ::
+            { IsAllocated(heap, heap[o,f]) } // Trigger
+        IsHeap(heap) ==> IsAllocated(heap, heap[o,f]));
 
-function new([ref,name]any) returns (ref);
-function X([ref,name]any) returns ([ref,name]any);
+//function new([ref,<x>name]x) returns (ref);
+//function X([ref,<x>name]x) returns ([ref,<x>name]x);
 
-axiom (forall h:[ref,name]any :: 
-	{IsAllocated(X(h),new(h))} 
-	IsAllocated(X(h),new(h)));
+//axiom (forall h:[ref,<x>name]x :: 
+//	{IsAllocated(X(h),new(h))} 
+//	IsAllocated(X(h),new(h)));
 
-axiom (forall h:[ref,name]any :: 
-	!IsAllocated(h,new(h)));
+//axiom (forall h:[ref,<x>name]x :: 
+//	!IsAllocated(h,new(h)));
 
-axiom (forall h:[ref,name]any, o:ref, f:name :: 
-	{X(h)[o,f]}
-	IsAllocated(h,o) ==> (X(h)[o,f] == h[o,f]));
+//axiom (forall h:[ref,<x>name]x, o:ref, f:name :: 
+//	{X(h)[o,f]}
+//	IsAllocated(h,o) ==> (X(h)[o,f] == h[o,f]));
 
 // Void are always allocated
-axiom (forall h: [ref,name]any :: 
-	{ IsAllocated(h,null) } 
-	IsAllocated(h,null));
+axiom (forall heap: [ref,<x>name]x :: 
+            { IsAllocated(heap, null) } // Trigger
+        IsAllocated(heap, null));
 
 // The global heap is a heap
-var Heap: [ref,name]any where IsHeap(Heap);
+var Heap: [ref,<x>name]x where IsHeap(Heap);
+
+
+// ----------------------------------------------------------------------
+// Function call checks
+
+// Only objects which are not null and are allocated are valid to call.
+// Assert this function before every regular feature call.
+function ValidCallTarget(heap: [ref,<x>name]x, o: ref) returns (bool);
+axiom (forall heap: [ref,<x>name]x, o: ref ::
+            { ValidCallTarget(heap, o) } // Trigger
+        IsHeap(heap) ==> (ValidCallTarget(heap, o) <==> o != null && heap[o, $allocated]));
+
+// Only objects which are not null and are not yet allocated are valid for
+// creation. Assert this function before every call to a creation feature.
+function ValidCreateTarget(heap: [ref,<x>name]x, o: ref) returns (bool);
+axiom (forall heap: [ref,<x>name]x, o: ref  ::
+            { ValidCreateTarget(heap, o) } // Trigger
+        IsHeap(heap) ==> (ValidCreateTarget(heap, o) <==> o != null && !heap[o, $allocated]));
+
+// Created objects need to be allocated on the heap. Assert this function
+// after every call to a creation feature.
+function ValidCreation(heap: [ref,<x>name]x, o: ref) returns (bool);
+axiom (forall heap: [ref,<x>name]x, o: ref  ::
+            { ValidCreation(heap, o) } // Trigger
+        IsHeap(heap) ==> (ValidCreation(heap, o) <==> o != null && heap[o, $allocated]));
+
 
 // ----------------------------------------------------------------------
 // set theory
@@ -159,8 +186,8 @@ axiom (forall s1:set,s2:set :: {set.difference(s1,s2)}
 // ----------------------------------------------------------------------
 // ANY functions
 
-function fun.ANY.conforms_to([ref,name]any,any,any) returns (bool);
-axiom (forall h:[ref,name]any,a:ref,b:ref :: { fun.ANY.conforms_to(h,a,b) }
+function fun.ANY.conforms_to([ref,<x>name]x,any,any) returns (bool);
+axiom (forall h:[ref,<x>name]x,a:ref,b:ref :: { fun.ANY.conforms_to(h,a,b) }
 	fun.ANY.conforms_to(h,a,b) == true);
 
 // ----------------------------------------------------------------------
@@ -172,16 +199,16 @@ axiom (forall c:int :: { int.abs(c) } (c >= 0) ==> (int.abs(c) == c));
 axiom (forall c:int :: { int.abs(c) } (c <= 0) ==> (int.abs(c) == -c));
 
 // out
-function fun.INTEGER_32.out([ref,name]any,int) returns (ref);
-axiom (forall h:[ref,name]any,c:int :: { fun.INTEGER_32.out(h,c) }
+function fun.INTEGER_32.out([ref,<x>name]x,int) returns (ref);
+axiom (forall h:[ref,<x>name]x,c:int :: { fun.INTEGER_32.out(h,c) }
 	(fun.INTEGER_32.out(h,c) != null));
 
 // ----------------------------------------------------------------------
 // BOOLEAN functions
 
 // out
-function fun.BOOLEAN.out([ref,name]any,int) returns (ref);
-axiom (forall h:[ref,name]any,c:int :: { fun.BOOLEAN.out(h,c) }
+function fun.BOOLEAN.out([ref,<x>name]x,int) returns (ref);
+axiom (forall h:[ref,<x>name]x,c:int :: { fun.BOOLEAN.out(h,c) }
 	(fun.BOOLEAN.out(h,c) != null));
 
 // ----------------------------------------------------------------------
@@ -200,5 +227,97 @@ function any_string (int) returns (ref);
 // FRAME functions
 
 
+// ----------------------------------------------------------------------
+// ROUTINE functions
+
+// Precondition, closed target, 1 argument
+function fun.ROUTINE.precondition(heap: [ref,<x>name]x, agent: ref, arg: any) returns (bool);
+
+// Postcondition, closed target, 1 argument
+function fun.ROUTINE.postcondition(heap: [ref,<x>name]x, agent: ref, arg: any) returns (bool);
+
+// Agent call
+procedure proc.ROUTINE.call (
+        Current: ref where Current != null && Heap[Current,$allocated],     // The agent object
+        arg: any);
+    requires fun.ROUTINE.precondition(Heap, Current, arg);
+    modifies Heap;
+    ensures fun.ROUTINE.postcondition(Heap, Current, arg);
+
+// Pseudo-attribute `feature' for agents
+// Denotes the name of the feature which an agent represents
+const unique $feature: <name>name;
+
+// Attribute `target' of class ROUTINE
+const unique field.ROUTINE.target: <ref>name;
+
+// Function `target' of class ROUTINE
+function fun.ROUTINE.target(heap: [ref, <x>name]x, agent: ref) returns (ref);
+axiom (forall heap:[ref, <x>name]x, agent:ref ::
+            { fun.ROUTINE.target(heap, agent) } // Trigger
+        IsHeap(heap) ==> (fun.ROUTINE.target(heap, agent) == heap[agent, field.ROUTINE.target]));
+
+// Creation feature
+procedure create.ROUTINE.create_with_target(
+        Current: ref where Current != null && !Heap[Current,$allocated],    // The agent object
+        feature: name,                                                      // The name of the associated feature
+        target: ref);                                                       // The closed target object
+    // Precondition: valid target object
+    requires target != null && Heap[target,$allocated];
+    modifies Heap;
+    // Postcondition: target set
+    ensures fun.ROUTINE.target(Heap, Current) == target;
+    // Frame condition
+    ensures (forall $o: ref, $f: name :: { Heap[$o, $f] } $o != null && old(Heap)[$o, $allocated] && $o != Current ==> old(Heap)[$o, $f] == Heap[$o, $f]);
+    // Object allocated
+    free ensures Heap[Current, $allocated];
+    // Feature association set
+    free ensures Heap[Current, $feature] == feature;
+
+
+
+// The actual precondition of an agent.
+// Add axioms for all features which are used as an agent
+function actual_precondition(feature: name, heap: [ref, <x>name]x, agent: ref, arg: ref) returns (bool);
+
+// The actual postcondition of an agent.
+// Add axioms for all features which are used as an agent
+function actual_postcondition(feature: name, heap: [ref, <x>name]x, agent: ref, arg: ref) returns (bool);
+
+
+// Associate general precondition of an agent with the actual precondition
+axiom (forall heap: [ref, <x>name]x, agent: ref, arg: ref :: 
+            { fun.ROUTINE.precondition(heap, agent, arg) } // Trigger
+        IsHeap(heap) ==> (fun.ROUTINE.precondition(heap, agent, arg) <==> actual_precondition(heap[agent,$feature], heap, agent, arg) ));
+
+// Associate general postcondition of an agent with the actual postcondition
+axiom (forall heap: [ref, <x>name]x, agent: ref, arg: ref :: 
+            { fun.ROUTINE.postcondition(heap, agent, arg) } // Trigger
+        IsHeap(heap) ==> (fun.ROUTINE.postcondition(heap, agent, arg) <==> actual_postcondition(heap[agent,$feature], heap, agent, arg) ));
+
+  
 // Background theory ends here
 // ======================================================================
+
+
+// **********************************************************************
+
+// Feature {FORMATTER}.align_left
+const unique feature.FORMATTER.align_left: name;
+axiom (forall heap: [ref, <x>name]x, agent: ref, arg: ref ::
+            { actual_precondition(feature.FORMATTER.align_left, heap, agent, arg) } // Trigger
+        actual_precondition(feature.FORMATTER.align_left, heap, agent, arg) <==> arg != null && !fun.PARAGRAPH.is_left_aligned(heap, arg));
+axiom (forall heap: [ref, <x>name]x, agent: ref, arg: ref ::
+            { actual_postcondition(feature.FORMATTER.align_left, heap, agent, arg) } // Trigger
+        actual_postcondition(feature.FORMATTER.align_left, heap, agent, arg) <==> fun.PARAGRAPH.is_left_aligned(heap, arg));
+
+// Feature {FORMATTER}.align_right
+const unique feature.FORMATTER.align_right: name;
+axiom (forall heap: [ref, <x>name]x, agent: ref, arg: ref ::
+            { actual_precondition(feature.FORMATTER.align_right, heap, agent, arg) } // Trigger
+        actual_precondition(feature.FORMATTER.align_right, heap, agent, arg) <==> arg != null && fun.PARAGRAPH.is_left_aligned(heap, arg));
+axiom (forall heap: [ref, <x>name]x, agent: ref, arg: ref ::
+            { actual_postcondition(feature.FORMATTER.align_right, heap, agent, arg) } // Trigger
+        actual_postcondition(feature.FORMATTER.align_right, heap, agent, arg) <==> !fun.PARAGRAPH.is_left_aligned(heap, arg));
+
+// **********************************************************************
