ballet/63/Src/Eiffel/eiffel/AST/visitor/ast_feature_checker_generator.e
@@ -527,6 +527,9 @@ feature {NONE} -- Implementation: State
 	is_checking_cas: BOOLEAN
 			-- Is a custom attribute being processed?
 
+	is_checking_frame: BOOLEAN
+			-- Is a frame expression being processed?
+
 	error_level: NATURAL_32 is
 			-- Convenience feature for compactness.
 		do
@@ -704,6 +707,14 @@ feature -- Settings
 			end
 		ensure
 			is_in_assignment_set: is_in_assignment = b
+		end
+
+	set_is_checking_frame (b: BOOLEAN) is
+			-- Assign `b' to `is_checking_frame'.
+		do
+			is_checking_frame := b
+		ensure
+			is_in_frame: is_checking_frame = b
 		end
 
 	set_current_feature (a_feature: FEATURE_I) is
@@ -3025,6 +3036,33 @@ feature -- Implementation
 						-- Result is not properly initialized.
 					error_handler.insert_error (create {VEVI}.make_result (context, l_as.end_keyword))
 				end
+
+					-- Check use frame
+				if l_as.use_frame /= Void then
+					-- TODO check, that old, Result are not in frame expressions
+					set_is_checking_frame(True)
+					l_as.use_frame.process (Current)
+					if l_needs_byte_node then
+						l_list ?= last_byte_node
+						l_byte_code.set_use_frame (l_list)
+					end
+					-- reset the levels to default values
+					set_is_checking_frame(False)
+				end
+
+					-- Check modify frame
+				if l_as.modify_frame /= Void then
+					set_is_checking_frame(True)
+					l_as.modify_frame.process (Current)
+					if l_needs_byte_node then
+						l_list ?= last_byte_node
+						l_byte_code.set_modify_frame (l_list)
+					end
+					-- reset the levels to default values
+					set_is_checking_frame(False)
+				end
+
+
 --				if is_creation_procedure then
 --						-- Verify that attributes are properly initialized.
 --					from
@@ -3219,6 +3257,7 @@ feature -- Implementation
 			l_assert: ASSERT_B
 			l_expr: EXPR_B
 			l_error_level: NATURAL_32
+			l_frame: FRAME_B
 		do
 			break_point_slot_count := break_point_slot_count + 1
 
@@ -3228,27 +3267,52 @@ feature -- Implementation
 			l_as.expr.process (Current)
 
 			if error_level = l_error_level then
-					-- Check if the type of the expression is boolean
-				if not last_type.actual_type.is_boolean then
-					create l_vwbe3
-					context.init_error (l_vwbe3)
-					l_vwbe3.set_type (last_type)
-					l_vwbe3.set_location (l_as.expr.end_location)
-					error_handler.insert_error (l_vwbe3)
-				elseif is_byte_node_enabled then
-					l_expr ?= last_byte_node
-					check
-						l_expr_not_void: l_expr /= Void
+				if is_checking_frame then
+					-- TODO: allow a subtype of FRAME?
+					if not last_type.associated_class.name.is_equal("FRAME") then
+-- TODO: create some meaningful error
+--					create l_vwbe3
+--					context.init_error (l_vwbe3)
+--					l_vwbe3.set_type (last_type)
+--					l_vwbe3.set_location (l_as.expr.end_location)
+					--					error_handler.insert_error (l_vwbe3)
+-- TODO
+						io.put_string("Frame specification has wrong type:" + last_type.associated_class.name + "%N")
 					end
-					create l_assert
-					if l_as.tag /= Void then
-						l_assert.set_tag (l_as.tag.name)
-					else
-						l_assert.set_tag (Void)
+					if is_byte_node_enabled then
+						l_expr ?= last_byte_node
+						check
+							l_expr_not_void: l_expr /= Void
+						end
+						create l_frame
+						l_frame.set_tag (l_as.tag.name)
+						l_frame.set_expr (l_expr)
+						l_frame.set_line_number (l_as.expr.start_location.line)
+						last_byte_node := l_frame
 					end
-					l_assert.set_expr (l_expr)
-					l_assert.set_line_number (l_as.expr.start_location.line)
-					last_byte_node := l_assert
+				else
+						-- Check if the type of the expression is boolean
+					if not last_type.actual_type.is_boolean then
+						create l_vwbe3
+						context.init_error (l_vwbe3)
+						l_vwbe3.set_type (last_type)
+						l_vwbe3.set_location (l_as.expr.end_location)
+						error_handler.insert_error (l_vwbe3)
+					elseif is_byte_node_enabled then
+						l_expr ?= last_byte_node
+						check
+							l_expr_not_void: l_expr /= Void
+						end
+						create l_assert
+						if l_as.tag /= Void then
+							l_assert.set_tag (l_as.tag.name)
+						else
+							l_assert.set_tag (Void)
+						end
+						l_assert.set_expr (l_expr)
+						l_assert.set_line_number (l_as.expr.start_location.line)
+						last_byte_node := l_assert
+					end
 				end
 			end
 		end
@@ -3469,6 +3533,8 @@ feature -- Implementation
 				context.init_error (l_veen2a)
 				l_veen2a.set_location (l_as.start_location)
 				error_handler.insert_error (l_veen2a)
+				-- TODO: elseif is_checking_frame then
+				-- Result in frame
 			end
 			l_type := current_feature.type
 			create {TYPED_POINTER_A} last_type.make_typed (l_type)
@@ -9272,13 +9338,19 @@ feature {AST_EIFFEL} -- Frame conditions visitor
 	process_modify_as (l_as: MODIFY_AS) is
 			-- Process `l_as'.
 		do
-			-- TODO julian: implement
+			check is_checking_frame end
+			if l_as.assertions /= Void then
+				l_as.assertions.process (Current)
+			end
 		end
 
 	process_use_as (l_as: USE_AS) is
 			-- Process `l_as'.
 		do
-			-- TODO julian: implement
+			check is_checking_frame end
+			if l_as.assertions /= Void then
+				l_as.assertions.process (Current)
+			end
 		end
 
 
